A framework for proving concurrent safety with ghost state.
Committing before trying a different approach.

concurrency/JuicyMachineModule.v
@@ -41,16 +41,30 @@ Module THE_JUICY_MACHINE.
   Import JSEM.JuicyMachineLemmas.
 
   (* safety with ghost updates *)
-  Definition tp_bupd P tp :=
-    exists tid (cnt : JTP.containsThread tp tid), let phi := JTP.getThreadR cnt in
+  Definition tp_update tp phi tp' phi' :=
+    level phi' = level phi /\ resource_at phi' = resource_at phi /\
+    JSEM.join_all tp' phi' /\
+    exists (Hiff : forall t, JTP.containsThread tp' t <-> JTP.containsThread tp t),
+      (forall t (cnt : JTP.containsThread tp t), JTP.getThreadC cnt = JTP.getThreadC (proj2 (Hiff _) cnt) /\
+         level (JTP.getThreadR cnt) = level (JTP.getThreadR (proj2 (Hiff _) cnt)) /\
+         resource_at (JTP.getThreadR cnt) = resource_at (JTP.getThreadR (proj2 (Hiff _) cnt))) /\
+      JTP.lockGuts tp' = JTP.lockGuts tp /\ JTP.lockSet tp' = JTP.lockSet tp /\
+      JTP.lockRes tp' = JTP.lockRes tp /\ JTP.latestThread tp'= JTP.latestThread tp.
+
+  Lemma tp_update_refl : forall tp phi, JSEM.join_all tp phi -> tp_update tp phi tp phi.
+  Proof.
+    repeat split; auto.
+    unshelve eexists; [reflexivity|].
+    split; auto; intros.
+    replace (proj2 _ _) with cnt by apply proof_irr; auto.
+  Qed.
+
+  Definition tp_bupd P (tp : jstate) := forall phi, JSEM.join_all tp phi ->
     forall c : ghost,
      joins (ghost_of phi) (ghost_fmap (approx (level phi)) (approx (level phi)) c) ->
      exists b : ghost,
        joins b (ghost_fmap (approx (level phi)) (approx (level phi)) c) /\
-       exists phi' : rmap,
-         level phi' = level phi /\
-         resource_at phi' = resource_at phi /\ ghost_of phi' = b /\
-         P (JTP.updThreadR cnt phi').
+       exists phi' tp', tp_update tp phi tp' phi' /\ ghost_of phi' = b /\ P tp'.
 
   Inductive jm_csafe (ge : SEM.G) (st : jmachine_state) (m : mem) : nat -> Prop :=
   | Safe_0 : jm_csafe ge st m 0
